LoCalSafety.v
@@ -10,6 +10,7 @@ From Stdlib Require Import List.
 Import ListNotations.
 From Stdlib Require Import Strings.String.
 From Stdlib Require Import PeanoNat.
+From Stdlib Require Import Lia.
 From LocalMech Require Import LoCalSyntax.
 From LocalMech Require Import LoCalStatic.
 From LocalMech Require Import LoCalDynamic.
@@ -139,7 +140,13 @@ Definition alloc_wf
      (r ↦ ∅) ∈ A  ⟹  r ∉ dom(S) *)
   (forall r,
     In (r, AP_None) A ->
-    store_find_heap S r = None).
+    store_find_heap S r = None)
+  /\
+  (* Rule 5 — store-region-scoped:
+     any region with allocated cells is tracked by A with a current focus. *)
+  (forall r,
+    store_find_heap S r <> None ->
+    exists l, In (r, AP_Loc (l, r)) A).
 
 (* ================================================================= *)
 (* Store well-formedness  (main judgment)                             *)
@@ -315,6 +322,125 @@ Qed.
 Definition tenv_equiv (G1 G2 : type_env) : Prop :=
   forall x, lookup_tenv G1 x = lookup_tenv G2 x.
 
+Definition store_extends (Sigma Sigma' : store_type) : Prop :=
+  forall lr tc, In (lr, tc) Sigma -> In (lr, tc) Sigma'.
+
+Definition conloc_extends (C C' : conloc_env) : Prop :=
+  forall lr le, In (lr, le) C -> In (lr, le) C'.
+
+Lemma store_extends_refl :
+  forall Sigma,
+    store_extends Sigma Sigma.
+Proof.
+  unfold store_extends. auto.
+Qed.
+
+Lemma conloc_extends_refl :
+  forall C,
+    conloc_extends C C.
+Proof.
+  unfold conloc_extends. auto.
+Qed.
+
+Lemma in_remove_alloc_region_preserved :
+  forall A r r' ap',
+    In (r', ap') A ->
+    r' <> r ->
+    In (r', ap') (remove_alloc_region A r).
+Proof.
+  intros A r r' ap' Hin Hneq.
+  unfold remove_alloc_region.
+  induction A as [| [ra apa] A IH]; simpl in *.
+  - contradiction.
+  - destruct Hin as [Heq | Hin].
+    + inversion Heq; subst.
+      destruct (region_var_eq_dec r' r).
+      * contradiction.
+      * simpl. left. reflexivity.
+    + destruct (region_var_eq_dec ra r).
+      * apply IH; assumption.
+      * simpl. right. apply IH; assumption.
+Qed.
+
+Lemma in_remove_alloc_region_inv :
+  forall A r r' ap',
+    In (r', ap') (remove_alloc_region A r) ->
+    In (r', ap') A /\ r' <> r.
+Proof.
+  induction A as [| [ra apa] A IH]; intros r r' ap' Hin; simpl in Hin.
+  - contradiction.
+  - destruct (region_var_eq_dec ra r).
+    + destruct (IH _ _ _ Hin) as [HinA Hneq].
+      split.
+      * right. exact HinA.
+      * exact Hneq.
+    + destruct Hin as [Heq | Hin].
+      * inversion Heq; subst.
+        split.
+        -- left. reflexivity.
+        -- exact n.
+      * destruct (IH _ _ _ Hin) as [HinA Hneq].
+        split.
+        -- right. exact HinA.
+        -- exact Hneq.
+Qed.
+
+Lemma in_extend_alloc_new :
+  forall A r ap,
+    In (r, ap) (extend_alloc A r ap).
+Proof.
+  intros A r ap. unfold extend_alloc. simpl. left. reflexivity.
+Qed.
+
+Lemma in_extend_alloc_old :
+  forall A r ap r' ap',
+    In (r', ap') A ->
+    r' <> r ->
+    In (r', ap') (extend_alloc A r ap).
+Proof.
+  intros A r ap r' ap' Hin Hneq.
+  unfold extend_alloc. simpl. right.
+  apply in_remove_alloc_region_preserved; assumption.
+Qed.
+
+Lemma in_extend_nursery_inv :
+  forall N lr lr',
+    In lr' (extend_nursery N lr) ->
+    lr' = lr \/ In lr' N.
+Proof.
+  intros N lr lr' Hin.
+  simpl in Hin. destruct Hin as [Heq | Hin].
+  - left. symmetry. exact Heq.
+  - right. exact Hin.
+Qed.
+
+Lemma not_in_extend_nursery_inv :
+  forall N lr lr',
+    ~ In lr' (extend_nursery N lr) ->
+    lr' <> lr /\ ~ In lr' N.
+Proof.
+  intros N lr lr' Hnin.
+  split.
+  - intro Heq. apply Hnin. simpl. left. symmetry. exact Heq.
+  - intro Hin. apply Hnin. simpl. right. exact Hin.
+Qed.
+
+Lemma fresh_region_store_absent :
+  forall DI A N M S r,
+    alloc_wf DI A N M S ->
+    fresh_region A r ->
+    store_find_heap S r = None.
+Proof.
+  intros DI A N M S r Halloc Hfresh.
+  destruct Halloc as [_ [_ [_ [Hempty Htracked]]]].
+  destruct (store_find_heap S r) eqn:Hheap; auto.
+  exfalso.
+  assert (Hheap_ne : store_find_heap S r <> None).
+  { rewrite Hheap. discriminate. }
+  destruct (Htracked r Hheap_ne) as [l Hin].
+  exact (Hfresh (AP_Loc (l, r)) Hin).
+Qed.
+
 Definition subst_pat_val (x : term_var) (s : val) (p : pat) : pat :=
   match p with
   | pat_clause K binds body =>
@@ -441,6 +567,39 @@ Proof.
   - econstructor. eauto.
 Qed.
 
+Lemma value_typing_any_context :
+  forall FDs DI G Sigma C A N vl T,
+    has_type FDs DI G Sigma C A N A N (e_val vl) T ->
+    forall G' Sigma' C' A' N',
+      tenv_equiv G G' ->
+      (forall lr tc, In (lr, tc) Sigma -> In (lr, tc) Sigma') ->
+      has_type FDs DI G' Sigma' C' A' N' A' N' (e_val vl) T.
+Proof.
+  intros FDs DI G Sigma C A N vl T Hty.
+  inversion Hty; subst; intros G' Sigma' C' A' N' Heq Hsigma.
+  - apply T_Var.
+    + match goal with
+      | [ Hlk : lookup_tenv G x = Some _ |- _ ] =>
+          rewrite <- (Heq x); exact Hlk
+      end.
+    + match goal with
+      | [ Hstore : In ((l, r), tc) Sigma |- _ ] => apply Hsigma; exact Hstore
+      end.
+  - apply T_ConcreteLoc.
+    match goal with
+    | [ Hstore : In ((l, r), tc) Sigma |- _ ] => apply Hsigma; exact Hstore
+    end.
+Qed.
+
+Lemma has_type_value_same_io :
+  forall FDs DI G Sigma C A N A' N' vl T,
+    has_type FDs DI G Sigma C A N A' N' (e_val vl) T ->
+    A' = A /\ N' = N.
+Proof.
+  intros FDs DI G Sigma C A N A' N' vl T Hty.
+  inversion Hty; subst; auto.
+Qed.
+
 Scheme has_type_ind' := Induction for has_type Sort Prop
 with field_vals_have_type_ind' := Induction for field_vals_have_type Sort Prop
 with app_vals_have_type_ind' := Induction for app_vals_have_type Sort Prop
@@ -449,6 +608,257 @@ with pats_have_type_ind' := Induction for pats_have_type Sort Prop.
 
 Combined Scheme typing_mutind
   from has_type_ind', pat_has_type_ind', pats_have_type_ind'.
+
+(* The thesis treats fresh location/region binders as an implicit
+   side-condition.  We keep the typing rules monotone, and instead
+   expose the needed binder-freshness obligations as a separate
+   proof-side judgment that mirrors the typing derivation shape. *)
+Inductive has_type_fresh :
+  fun_env -> datacon_info ->
+  type_env -> store_type -> conloc_env ->
+  alloc_env -> nursery ->
+  alloc_env -> nursery ->
+  expr -> located_type -> Prop :=
+  | TF_Var :
+      forall FDs DI G Sigma C A N x tc l r,
+        has_type_fresh FDs DI G Sigma C A N A N
+                       (e_val (v_var x)) (LocTy tc l r)
+  | TF_ConcreteLoc :
+      forall FDs DI G Sigma C A N r0 i l r tc,
+        has_type_fresh FDs DI G Sigma C A N A N
+                       (e_val (v_cloc r0 i l r)) (LocTy tc l r)
+  | TF_Let :
+      forall FDs DI G Sigma C A N A' N' A'' N''
+             x e1 e2 tc1 l1 r1 tc2 l2 r2,
+        has_type_fresh FDs DI G Sigma C A N A' N' e1 (LocTy tc1 l1 r1) ->
+        has_type_fresh FDs DI (extend_tenv G x (LocTy tc1 l1 r1))
+                       (extend_store Sigma (l1, r1) tc1)
+                       C A' N' A'' N'' e2 (LocTy tc2 l2 r2) ->
+        has_type_fresh FDs DI G Sigma C A N A'' N''
+                       (ELet x (LocTy tc1 l1 r1) e1 e2) (LocTy tc2 l2 r2)
+  | TF_LRegion :
+      forall FDs DI G Sigma C A N A' N' r e t,
+        fresh_region A r ->
+        has_type_fresh FDs DI G Sigma C (extend_alloc A r AP_None) N A' N' e t ->
+        has_type_fresh FDs DI G Sigma C A N A' N' (e_letregion r e) t
+  | TF_LLStart :
+      forall FDs DI G Sigma C A N A'' N'' l r e tc' l' r',
+        letloc_fresh_ctx Sigma C A N (l, r) ->
+        has_type_fresh FDs DI G Sigma
+                       (extend_conloc C (l, r) (LE_Start r))
+                       (extend_alloc A r (AP_Loc (l, r)))
+                       (extend_nursery N (l, r))
+                       A'' N'' e (LocTy tc' l' r') ->
+        has_type_fresh FDs DI G Sigma C A N A'' N''
+                       (e_letloc l r (LE_Start r) e) (LocTy tc' l' r')
+  | TF_LLTag :
+      forall FDs DI G Sigma C A N A'' N'' l lprev r e tc'' l'' r'',
+        letloc_fresh_ctx Sigma C A N (l, r) ->
+        has_type_fresh FDs DI G Sigma
+                       (extend_conloc C (l, r) (LE_Next lprev r))
+                       (extend_alloc A r (AP_Loc (l, r)))
+                       (extend_nursery N (l, r))
+                       A'' N'' e (LocTy tc'' l'' r'') ->
+        has_type_fresh FDs DI G Sigma C A N A'' N''
+                       (e_letloc l r (LE_Next lprev r) e) (LocTy tc'' l'' r'')
+  | TF_LLAfter :
+      forall FDs DI G Sigma C A N A'' N'' l l1 r tc_prev e tc' l' r',
+        letloc_fresh_ctx Sigma C A N (l, r) ->
+        has_type_fresh FDs DI G Sigma
+                       (extend_conloc C (l, r) (LE_After tc_prev l1 r))
+                       (extend_alloc A r (AP_Loc (l, r)))
+                       (extend_nursery N (l, r))
+                       A'' N'' e (LocTy tc' l' r') ->
+        has_type_fresh FDs DI G Sigma C A N A'' N''
+                       (e_letloc l r (LE_After tc_prev l1 r) e) (LocTy tc' l' r')
+  | TF_DataCon :
+      forall FDs DI G Sigma C A N dc l r vs tc
+             (fieldtcs : list tycon) (fields : list field_layout_entry),
+        has_type_fresh FDs DI G Sigma C A N
+                       (extend_alloc A r (AP_Loc (l, r)))
+                       (remove_nursery N (l, r))
+                       (e_datacon dc l r vs) (LocTy tc l r)
+  | TF_App :
+      forall FDs DI G Sigma C A N f lrs vs tc l r
+             (f_locs : list (loc_var * region_var))
+             (f_params : list (term_var * ty))
+             (f_retty : ty)
+             (f_regions : list region_var)
+             (f_body : expr),
+        has_type_fresh FDs DI G Sigma C A N A
+                       (remove_nursery N (l, r))
+                       (e_app f lrs vs) (LocTy tc l r)
+  | TF_Case :
+      forall FDs DI G Sigma C A N A' N' scrut ps tc_s
+             (l_s : loc_var) (r_s : region_var) t,
+        pats_have_type_fresh FDs DI tc_s G Sigma C A N A' N' t ps ->
+        has_type_fresh FDs DI G Sigma C A N A' N'
+                       (e_case scrut ps) t
+
+with pat_has_type_fresh :
+  fun_env -> datacon_info ->
+  tycon -> type_env -> store_type -> conloc_env ->
+  alloc_env -> nursery ->
+  alloc_env -> nursery ->
+  located_type -> pat -> Prop :=
+  | TF_Pat :
+      forall FDs DI tc_s G Sigma C A N A' N'
+             dc binds body (tc : tycon) (fieldtcs : list tycon)
+             (tc_res : tycon) (l : loc_var) (r : region_var),
+        has_type_fresh FDs DI
+                       (extend_tenv_list G binds)
+                       (extend_store_list Sigma (pat_store_entries binds))
+                       C A N A' N' body (LocTy tc_res l r) ->
+        pat_has_type_fresh FDs DI tc_s G Sigma C A N A' N'
+                           (LocTy tc_res l r) (pat_clause dc binds body)
+
+with pats_have_type_fresh :
+  fun_env -> datacon_info ->
+  tycon -> type_env -> store_type -> conloc_env ->
+  alloc_env -> nursery ->
+  alloc_env -> nursery ->
+  located_type -> list pat -> Prop :=
+  | TF_PatsNil :
+      forall FDs DI tc_s G Sigma C A N t,
+        pats_have_type_fresh FDs DI tc_s G Sigma C A N A N t nil
+  | TF_PatsCons :
+      forall FDs DI tc_s G Sigma C A N A1 N1 A2 N2 t p ps,
+        pat_has_type_fresh FDs DI tc_s G Sigma C A N A1 N1 t p ->
+        pats_have_type_fresh FDs DI tc_s G Sigma C A1 N1 A2 N2 t ps ->
+        pats_have_type_fresh FDs DI tc_s G Sigma C A N A2 N2 t (cons p ps).
+
+Scheme has_type_fresh_ind' := Induction for has_type_fresh Sort Prop
+with pat_has_type_fresh_ind' := Induction for pat_has_type_fresh Sort Prop
+with pats_have_type_fresh_ind' := Induction for pats_have_type_fresh Sort Prop.
+
+Lemma lookup_loc_extend_eq :
+  forall M lr cl,
+    lookup_loc (extend_loc M lr cl) lr = Some cl.
+Proof.
+  intros M lr cl.
+  unfold extend_loc. simpl.
+  destruct (laddr_eq_dec lr lr); congruence.
+Qed.
+
+Lemma lookup_loc_extend_neq :
+  forall M lr1 lr2 cl,
+    lr1 <> lr2 ->
+    lookup_loc (extend_loc M lr2 cl) lr1 = lookup_loc M lr1.
+Proof.
+  intros M lr1 lr2 cl Hneq.
+  unfold extend_loc. simpl.
+  destruct (laddr_eq_dec lr1 lr2); congruence.
+Qed.
+
+Lemma in_store_laddrs_of_entry :
+  forall Sigma lr tc,
+    In (lr, tc) Sigma ->
+    In lr (store_laddrs Sigma).
+Proof.
+  induction Sigma as [| [lr' tc'] Sigma IH]; intros lr tc Hin.
+  - inversion Hin.
+  - simpl in *. destruct Hin as [Heq | Hin].
+    + inversion Heq; subst. simpl. left. reflexivity.
+    + simpl. right. eapply IH. exact Hin.
+Qed.
+
+Lemma in_conloc_support_of_key :
+  forall C lr le,
+    In (lr, le) C ->
+    In lr (conloc_support C).
+Proof.
+  induction C as [| [lr' le'] C IH]; intros lr le Hin.
+  - inversion Hin.
+  - simpl in *. destruct Hin as [Heq | Hin].
+    + inversion Heq; subst. simpl. left. reflexivity.
+    + simpl. right. apply in_or_app. right. eapply IH. exact Hin.
+Qed.
+
+Lemma in_conloc_support_of_rhs :
+  forall C lr lr' le,
+    In (lr', le) C ->
+    In lr (locexp_laddrs le) ->
+    In lr (conloc_support C).
+Proof.
+  induction C as [| [lr0 le0] C IH]; intros lr lr' le HinC HinLe.
+  - inversion HinC.
+  - simpl in *. destruct HinC as [Heq | HinC].
+    + inversion Heq; subst. simpl. right. apply in_or_app. left. exact HinLe.
+    + simpl. right. apply in_or_app. right.
+      apply IH with (lr' := lr') (le := le); assumption.
+Qed.
+
+Lemma in_alloc_laddrs_of_entry :
+  forall A r lr,
+    In (r, AP_Loc lr) A ->
+    In lr (alloc_laddrs A).
+Proof.
+  induction A as [| [r' ap] A IH]; intros r lr Hin.
+  - inversion Hin.
+  - simpl in *. destruct Hin as [Heq | Hin].
+    + inversion Heq; subst. simpl. left. reflexivity.
+    + destruct ap; simpl.
+      * eapply IH. exact Hin.
+      * right. eapply IH. exact Hin.
+Qed.
+
+Lemma max_heap_index_none_nil :
+  forall h,
+    max_heap_index h = None ->
+    h = nil.
+Proof.
+  induction h as [| [i K] h IH]; intros Hmax.
+  - reflexivity.
+  - simpl in Hmax. destruct (max_heap_index h); discriminate.
+Qed.
+
+Lemma heap_find_gt_max_none :
+  forall h i k,
+    max_heap_index h = Some k ->
+    i > k ->
+    heap_find h i = None.
+Proof.
+  induction h as [| [j K] h IH]; intros i k Hmax Hgt.
+  - inversion Hmax.
+  - simpl in Hmax.
+    destruct (max_heap_index h) as [k'|] eqn:Hmax_tl.
+    + inversion Hmax; subst k. simpl.
+      assert (Hij : i <> j) by lia.
+      destruct (Nat.eqb i j) eqn:Heq; [apply Nat.eqb_eq in Heq; contradiction|].
+      apply (IH i k').
+      * reflexivity.
+      * lia.
+    + apply max_heap_index_none_nil in Hmax_tl. subst h.
+      inversion Hmax; subst k. simpl.
+      assert (Hij : i <> j) by lia.
+      destruct (Nat.eqb i j) eqn:Heq; [apply Nat.eqb_eq in Heq; contradiction|].
+      reflexivity.
+Qed.
+
+Lemma gt_allocptr_heap_lookup_none :
+  forall S r i,
+    gt_allocptr i (allocptr S r) ->
+    heap_lookup S r i = None.
+Proof.
+  intros S r i Hgt.
+  unfold allocptr, heap_lookup in *.
+  destruct (store_find_heap S r) as [h|] eqn:Hheap; simpl in *.
+  - destruct (max_heap_index h) as [k|] eqn:Hmax.
+    + eapply heap_find_gt_max_none; eauto.
+    + apply max_heap_index_none_nil in Hmax. subst h. reflexivity.
+  - reflexivity.
+Qed.
+
+Lemma gt_allocptr_succ :
+  forall i ap,
+    gt_allocptr i ap ->
+    gt_allocptr (i + 1) ap.
+Proof.
+  intros i ap Hgt.
+  destruct ap as [k|]; simpl in *.
+  - lia.
+  - exact I.
+Qed.
 
 Lemma has_type_tenv_equiv :
   (forall FDs DI G Sigma C A N A' N' e T,
@@ -485,16 +895,17 @@ Proof.
     eapply T_Let.
     + apply IH1. exact Heq.
     + apply IH2. apply tenv_equiv_extend. exact Heq.
-  - intros FDs DI G S0 C A N A' N' r e t Hty IH G' Heq.
-    eapply T_LRegion. apply IH. exact Heq.
-  - intros FDs DI G S0 C A N A'' N'' l r e tc' l' r' Hnone Hfresh Hneq
-      Hty IH G' Heq.
+  - intros FDs DI G S0 C A N A' N' r e t Hfresh Hty IH G' Heq.
+    eapply T_LRegion; eauto.
+  - intros FDs DI G S0 C A N A'' N'' l r e tc' l' r'
+      Halloc HfreshOut Hneq Hty IH G' Heq.
     eapply T_LLStart; eauto.
   - intros FDs DI G S0 C A N A'' N'' l lprev r e tc'' l'' r''
-      Halloc Hnur Hfresh Hneq Hty IH G' Heq.
+      Halloc Hnur HfreshOut Hneq Hty IH G' Heq.
     eapply T_LLTag; eauto.
   - intros FDs DI G S0 C A N A'' N'' l l1 r tc_prev e tc' l' r'
-      Halloc Hstore Hnotin Hfresh Hneq Hty IH G' Heq.
+      Halloc Hstore Hnotin HfreshOut Hneq
+      Hty IH G' Heq.
     eapply T_LLAfter; eauto.
   - intros FDs DI G S0 C A N dc l r vs tc fieldtcs fields
       Hdc Hnur Hfields Hlayout Hfocus Hvals IHvals G' Heq.
@@ -560,6 +971,705 @@ Corollary pats_have_type_tenv_equiv :
 Proof.
   intros. destruct has_type_tenv_equiv as [_ [_ Hps]].
   eauto.
+Qed.
+
+Lemma store_extends_extend_store :
+  forall Sigma Sigma' lr tc,
+    store_extends Sigma Sigma' ->
+    store_extends (extend_store Sigma lr tc) (extend_store Sigma' lr tc).
+Proof.
+  intros Sigma Sigma' lr tc Hext lr' tc' Hin.
+  simpl in Hin. destruct Hin as [Heq | Hin].
+  - left. exact Heq.
+  - right. apply Hext. exact Hin.
+Qed.
+
+Lemma store_extends_extend_store_list :
+  forall Sigma Sigma' entries,
+    store_extends Sigma Sigma' ->
+    store_extends (extend_store_list Sigma entries)
+                  (extend_store_list Sigma' entries).
+Proof.
+  intros Sigma Sigma' entries.
+  revert Sigma Sigma'.
+  induction entries as [| ent entries IH]; intros Sigma Sigma' Hext; simpl.
+  - exact Hext.
+  - destruct ent as [lr0 tc0].
+    apply IH. apply store_extends_extend_store. exact Hext.
+Qed.
+
+Lemma conloc_extends_extend_conloc :
+  forall C C' lr le,
+    conloc_extends C C' ->
+    conloc_extends (extend_conloc C lr le) (extend_conloc C' lr le).
+Proof.
+  intros C C' lr le Hext lr' le' Hin.
+  simpl in Hin. destruct Hin as [Heq | Hin].
+  - left. exact Heq.
+  - right. apply Hext. exact Hin.
+Qed.
+
+Lemma constructor_layout_extends :
+  forall C C' root_l r prev_tc fields,
+    constructor_layout C root_l r prev_tc fields ->
+    conloc_extends C C' ->
+    constructor_layout C' root_l r prev_tc fields.
+Proof.
+  intros C C' root_l r prev_tc fields Hlayout Hext.
+  revert root_l prev_tc Hlayout.
+  induction fields as [| [lf tc] fields IH]; intros root_l prev_tc Hlayout; simpl in *.
+  - exact I.
+  - destruct Hlayout as [Hhd Htl]. split.
+    + destruct prev_tc.
+      * apply Hext. exact Hhd.
+      * apply Hext. exact Hhd.
+    + apply IH; assumption.
+Qed.
+
+Lemma store_wf_extend_store_existing :
+  forall DI Sigma C A N M S lr tc,
+    store_wf DI Sigma C A N M S ->
+    In (lr, tc) Sigma ->
+    store_wf DI (extend_store Sigma lr tc) C A N M S.
+Proof.
+  intros DI Sigma C A N M S lr tc Hwf Hin_old.
+  destruct Hwf as [Hmap [Hcfc [Halloc [Hdisj1 Hdisj2]]]].
+  destruct Hcfc as [Hstart [Hnext Hafter]].
+  destruct Halloc as [Hlin1 [Hlin2 [Hwrite [Hempty Htracked]]]].
+  repeat split.
+  - intros l r T Hin.
+    simpl in Hin. destruct Hin as [Heq | Hin].
+    + inversion Heq; subst. eapply Hmap. exact Hin_old.
+    + eapply Hmap. exact Hin.
+  - exact Hstart.
+  - exact Hnext.
+  - exact Hafter.
+  - exact Hlin1.
+  - exact Hlin2.
+  - exact Hwrite.
+  - exact Hempty.
+  - exact Htracked.
+  - intros l r T Hin.
+    simpl in Hin. destruct Hin as [Heq | Hin].
+    + inversion Heq; subst. eapply Hdisj1. exact Hin_old.
+    + eapply Hdisj1. exact Hin.
+  - intros l r HinN Hex.
+    simpl in Hex. destruct Hex as [T [Heq | Hin]].
+    + inversion Heq; subst. eapply Hdisj2; eauto.
+    + eapply Hdisj2; eauto.
+Qed.
+
+Lemma store_wf_extend_alloc_none_fresh :
+  forall DI Sigma C A N M S r,
+    store_wf DI Sigma C A N M S ->
+    fresh_region A r ->
+    store_wf DI Sigma C (extend_alloc A r AP_None) N M S.
+Proof.
+  intros DI Sigma C A N M S r Hwf Hfresh.
+  destruct Hwf as [Hmap [Hcfc [Halloc [Hdisj1 Hdisj2]]]].
+  destruct Hcfc as [Hstart [Hnext Hafter]].
+  destruct Halloc as [Hlin1 [Hlin2 [Hwrite [Hempty Htracked]]]].
+  assert (Hallocwf : alloc_wf DI A N M S).
+  { repeat split; assumption. }
+  repeat split.
+  - exact Hmap.
+  - exact Hstart.
+  - exact Hnext.
+  - exact Hafter.
+  - intros r' l HinA HinN.
+    destruct HinA as [Heq | HinA].
+    + inversion Heq.
+    + apply filter_In in HinA as [HinA _].
+      eapply Hlin1; eauto.
+  - intros r' l i T j HinA Hlk Hnin Hew.
+    destruct HinA as [Heq | HinA].
+    + inversion Heq.
+    + apply filter_In in HinA as [HinA _].
+      eapply Hlin2; eauto.
+  - exact Hwrite.
+  - intros r' HinA.
+    destruct HinA as [Heq | HinA].
+    + inversion Heq; subst.
+      exact (fresh_region_store_absent _ _ _ _ _ _ Hallocwf Hfresh).
+    + apply filter_In in HinA as [HinA _].
+      eapply Hempty; eauto.
+  - intros r' Hheap.
+    destruct (region_var_eq_dec r' r) as [Heq | Hneq].
+    + subst. exfalso.
+      rewrite (fresh_region_store_absent _ _ _ _ _ _ Hallocwf Hfresh) in Hheap.
+      contradiction.
+    + destruct (Htracked r' Hheap) as [l Hin].
+      exists l. eapply in_extend_alloc_old; eauto.
+  - exact Hdisj1.
+  - exact Hdisj2.
+Qed.
+
+Lemma store_wf_extend_letloc_start :
+  forall DI Sigma C A N M S l r,
+    store_wf DI Sigma C A N M S ->
+    letloc_fresh_ctx Sigma C A N (l, r) ->
+    In (r, AP_None) A ->
+    store_wf DI Sigma
+             (extend_conloc C (l, r) (LE_Start r))
+             (extend_alloc A r (AP_Loc (l, r)))
+             (extend_nursery N (l, r))
+             (extend_loc M (l, r) (r, 0))
+             S.
+Proof.
+  intros DI Sigma C A N M S l r Hwf Hfresh Hnone.
+  destruct Hfresh as [HfreshS [HfreshC [HfreshA HfreshN]]].
+  destruct Hwf as [Hmap [Hcfc [Halloc [Hdisj1 Hdisj2]]]].
+  destruct Hcfc as [Hstart [Hnext Hafter]].
+  destruct Halloc as [Hlin1 [Hlin2 [Hwrite [Hempty Htracked]]]].
+  repeat split.
+  - intros l0 r0 T HinSigma.
+    destruct (Hmap l0 r0 T HinSigma) as [i [j [Hlk Hew]]].
+    exists i, j. split.
+    + rewrite lookup_loc_extend_neq.
+      * exact Hlk.
+      * intro Heq. apply HfreshS. rewrite <- Heq.
+        eapply in_store_laddrs_of_entry. exact HinSigma.
+    + exact Hew.
+  - intros l0 r0 HinC.
+    simpl in HinC. destruct HinC as [Heq | HinC].
+    + inversion Heq; subst. apply lookup_loc_extend_eq.
+    + rewrite lookup_loc_extend_neq.
+      * eapply Hstart. exact HinC.
+      * intro Heq. apply HfreshC. rewrite <- Heq.
+        eapply in_conloc_support_of_key. exact HinC.
+  - intros l0 r0 lprev HinC.
+    simpl in HinC. destruct HinC as [Heq | HinC].
+    + inversion Heq.
+    + destruct (Hnext l0 r0 lprev HinC) as [i [Hsrc Hdst]].
+      exists i. split.
+      * rewrite lookup_loc_extend_neq.
+        -- exact Hsrc.
+        -- intro Heq. apply HfreshC. rewrite <- Heq.
+           eapply in_conloc_support_of_rhs with (lr' := (l0, r0)) (le := LE_Next lprev r0).
+           ++ exact HinC.
+           ++ simpl. left. reflexivity.
+      * rewrite lookup_loc_extend_neq.
+        -- exact Hdst.
+        -- intro Heq. apply HfreshC. rewrite <- Heq.
+           eapply in_conloc_support_of_key. exact HinC.
+  - intros l0 r0 T l1 HinC.
+    simpl in HinC. destruct HinC as [Heq | HinC].
+    + inversion Heq.
+    + destruct (Hafter l0 r0 T l1 HinC) as [i [j [Hsrc [Hew Hdst]]]].
+      exists i, j. repeat split.
+      * rewrite lookup_loc_extend_neq.
+        -- exact Hsrc.
+        -- intro Heq. apply HfreshC. rewrite <- Heq.
+           eapply in_conloc_support_of_rhs with (lr' := (l0, r0)) (le := LE_After T l1 r0).
+           ++ exact HinC.
+           ++ simpl. left. reflexivity.
+      * exact Hew.
+      * rewrite lookup_loc_extend_neq.
+        -- exact Hdst.
+        -- intro Heq. apply HfreshC. rewrite <- Heq.
+           eapply in_conloc_support_of_key. exact HinC.
+  - intros r0 l0 HinA HinN.
+    simpl in HinA. destruct HinA as [Heq | HinA].
+    + inversion Heq; subst. exists 0. split.
+      * apply lookup_loc_extend_eq.
+      * unfold gt_allocptr, allocptr.
+        rewrite (Hempty _ Hnone). reflexivity.
+    + destruct (in_remove_alloc_region_inv _ _ _ _ HinA) as [HinA_old _].
+      assert (Hneq_lr : (l0, r0) <> (l, r)).
+      { intro Heq. apply HfreshA. rewrite <- Heq.
+        eapply in_alloc_laddrs_of_entry. exact HinA_old. }
+      destruct (in_extend_nursery_inv N (l, r) (l0, r0) HinN) as [HeqN | HinN_old].
+      * contradiction.
+      * destruct (Hlin1 r0 l0 HinA_old HinN_old) as [i [Hlk Hgt]].
+        exists i. split.
+        -- rewrite lookup_loc_extend_neq.
+           ++ exact Hlk.
+           ++ exact Hneq_lr.
+        -- exact Hgt.
+  - intros r0 l0 i T j HinA Hlk Hnin Hew.
+    simpl in HinA. destruct HinA as [Heq | HinA].
+    + inversion Heq; subst. exfalso. apply Hnin. simpl. left. reflexivity.
+    + destruct (in_remove_alloc_region_inv _ _ _ _ HinA) as [HinA_old _].
+      assert (Hneq_lr : (l0, r0) <> (l, r)).
+      { intro Heq. apply HfreshA. rewrite <- Heq.
+        eapply in_alloc_laddrs_of_entry. exact HinA_old. }
+      destruct (not_in_extend_nursery_inv N (l, r) (l0, r0) Hnin) as [_ Hnin_old].
+      rewrite lookup_loc_extend_neq in Hlk by exact Hneq_lr.
+      eapply Hlin2; eauto.
+  - intros l0 r0 HinN.
+    destruct (in_extend_nursery_inv N (l, r) (l0, r0) HinN) as [Heq | HinN_old].
+    + inversion Heq; subst. exists 0. split.
+      * apply lookup_loc_extend_eq.
+      * unfold heap_lookup. rewrite (Hempty _ Hnone). reflexivity.
+    + assert (Hneq_lr : (l0, r0) <> (l, r)).
+      { intro Heq. apply HfreshN. rewrite Heq in HinN_old. exact HinN_old. }
+      destruct (Hwrite l0 r0 HinN_old) as [i [Hlk Hnone_cell]].
+      exists i. split.
+      * rewrite lookup_loc_extend_neq.
+        -- exact Hlk.
+        -- exact Hneq_lr.
+      * exact Hnone_cell.
+  - intros r0 HinA.
+    simpl in HinA. destruct HinA as [Heq | HinA].
+    + inversion Heq.
+    + destruct (in_remove_alloc_region_inv _ _ _ _ HinA) as [HinA_old _].
+      eapply Hempty. exact HinA_old.
+  - intros r0 Hheap.
+    destruct (region_var_eq_dec r0 r) as [Heq | Hneq].
+    + subst. exists l. apply in_extend_alloc_new.
+    + destruct (Htracked r0 Hheap) as [l0 HinA].
+      exists l0. eapply in_extend_alloc_old; eauto.
+  - intros l0 r0 T HinSigma HinN.
+    destruct (in_extend_nursery_inv N (l, r) (l0, r0) HinN) as [Heq | HinN_old].
+    + apply HfreshS. rewrite <- Heq. eapply in_store_laddrs_of_entry. exact HinSigma.
+    + eapply Hdisj1; eauto.
+  - intros l0 r0 HinN HexSigma.
+    destruct (in_extend_nursery_inv N (l, r) (l0, r0) HinN) as [Heq | HinN_old].
+    + destruct HexSigma as [T HinSigma].
+      apply HfreshS. rewrite <- Heq. eapply in_store_laddrs_of_entry. exact HinSigma.
+    + eapply Hdisj2; eauto.
+Qed.
+
+Lemma store_wf_extend_letloc_tag :
+  forall DI Sigma C A N M S l lprev r i,
+    store_wf DI Sigma C A N M S ->
+    letloc_fresh_ctx Sigma C A N (l, r) ->
+    In (r, AP_Loc (lprev, r)) A ->
+    In (lprev, r) N ->
+    lookup_loc M (lprev, r) = Some (r, i) ->
+    store_wf DI Sigma
+             (extend_conloc C (l, r) (LE_Next lprev r))
+             (extend_alloc A r (AP_Loc (l, r)))
+             (extend_nursery N (l, r))
+             (extend_loc M (l, r) (r, i + 1))
+             S.
+Proof.
+  intros DI Sigma C A N M S l lprev r i Hwf Hfresh Hfocus_prev Hnur_prev Hlookup_prev.
+  destruct Hfresh as [HfreshS [HfreshC [HfreshA HfreshN]]].
+  destruct Hwf as [Hmap [Hcfc [Halloc [Hdisj1 Hdisj2]]]].
+  destruct Hcfc as [Hstart [Hnext Hafter]].
+  destruct Halloc as [Hlin1 [Hlin2 [Hwrite [Hempty Htracked]]]].
+  assert (Hgt_prev : gt_allocptr i (allocptr S r)).
+  { destruct (Hlin1 r lprev Hfocus_prev Hnur_prev) as [i0 [Hlk0 Hgt0]].
+    rewrite Hlookup_prev in Hlk0. inversion Hlk0; subst. exact Hgt0. }
+  repeat split.
+  - intros l0 r0 T HinSigma.
+    destruct (Hmap l0 r0 T HinSigma) as [i0 [j [Hlk Hew]]].
+    exists i0, j. split.
+    + rewrite lookup_loc_extend_neq.
+      * exact Hlk.
+      * intro Heq. apply HfreshS. rewrite <- Heq.
+        eapply in_store_laddrs_of_entry. exact HinSigma.
+    + exact Hew.
+  - intros l0 r0 HinC.
+    simpl in HinC. destruct HinC as [Heq | HinC].
+    + inversion Heq.
+    + rewrite lookup_loc_extend_neq.
+      * eapply Hstart. exact HinC.
+      * intro Heq. apply HfreshC. rewrite <- Heq.
+        eapply in_conloc_support_of_key. exact HinC.
+  - intros l0 r0 lprev0 HinC.
+    simpl in HinC. destruct HinC as [Heq | HinC].
+    + inversion Heq; subst. exists i. split.
+      * rewrite lookup_loc_extend_neq.
+        -- exact Hlookup_prev.
+        -- intro Heq_lr. apply HfreshA. rewrite <- Heq_lr.
+           eapply in_alloc_laddrs_of_entry. exact Hfocus_prev.
+      * apply lookup_loc_extend_eq.
+    + destruct (Hnext l0 r0 lprev0 HinC) as [i0 [Hsrc Hdst]].
+      exists i0. split.
+      * rewrite lookup_loc_extend_neq.
+        -- exact Hsrc.
+        -- intro Heq. apply HfreshC. rewrite <- Heq.
+           eapply in_conloc_support_of_rhs
+             with (lr' := (l0, r0)) (le := LE_Next lprev0 r0).
+           ++ exact HinC.
+           ++ simpl. left. reflexivity.
+      * rewrite lookup_loc_extend_neq.
+        -- exact Hdst.
+        -- intro Heq. apply HfreshC. rewrite <- Heq.
+           eapply in_conloc_support_of_key. exact HinC.
+  - intros l0 r0 T l1 HinC.
+    simpl in HinC. destruct HinC as [Heq | HinC].
+    + inversion Heq.
+    + destruct (Hafter l0 r0 T l1 HinC) as [i0 [j [Hsrc [Hew Hdst]]]].
+      exists i0, j. repeat split.
+      * rewrite lookup_loc_extend_neq.
+        -- exact Hsrc.
+        -- intro Heq. apply HfreshC. rewrite <- Heq.
+           eapply in_conloc_support_of_rhs
+             with (lr' := (l0, r0)) (le := LE_After T l1 r0).
+           ++ exact HinC.
+           ++ simpl. left. reflexivity.
+      * exact Hew.
+      * rewrite lookup_loc_extend_neq.
+        -- exact Hdst.
+        -- intro Heq. apply HfreshC. rewrite <- Heq.
+           eapply in_conloc_support_of_key. exact HinC.
+  - intros r0 l0 HinA HinN.
+    simpl in HinA. destruct HinA as [Heq | HinA].
+    + inversion Heq; subst. exists (i + 1). split.
+      * apply lookup_loc_extend_eq.
+      * apply gt_allocptr_succ. exact Hgt_prev.
+    + destruct (in_remove_alloc_region_inv _ _ _ _ HinA) as [HinA_old Hrneq].
+      assert (Hneq_lr : (l0, r0) <> (l, r)).
+      { intro Heq. inversion Heq; subst. contradiction. }
+      destruct (in_extend_nursery_inv N (l, r) (l0, r0) HinN) as [HeqN | HinN_old].
+      * inversion HeqN; subst. contradiction.
+      * destruct (Hlin1 r0 l0 HinA_old HinN_old) as [i0 [Hlk Hgt]].
+        exists i0. split.
+        -- rewrite lookup_loc_extend_neq.
+           ++ exact Hlk.
+           ++ exact Hneq_lr.
+        -- exact Hgt.
+  - intros r0 l0 i0 T j HinA Hlk Hnin Hew.
+    simpl in HinA. destruct HinA as [Heq | HinA].
+    + inversion Heq; subst. exfalso. apply Hnin. simpl. left. reflexivity.
+    + destruct (in_remove_alloc_region_inv _ _ _ _ HinA) as [HinA_old _].
+      assert (Hneq_lr : (l0, r0) <> (l, r)).
+      { intro Heq. apply HfreshA. rewrite <- Heq.
+        eapply in_alloc_laddrs_of_entry. exact HinA_old. }
+      destruct (not_in_extend_nursery_inv N (l, r) (l0, r0) Hnin) as [_ Hnin_old].
+      rewrite lookup_loc_extend_neq in Hlk by exact Hneq_lr.
+      eapply Hlin2; eauto.
+  - intros l0 r0 HinN.
+    destruct (in_extend_nursery_inv N (l, r) (l0, r0) HinN) as [Heq | HinN_old].
+    + inversion Heq; subst. exists (i + 1). split.
+      * apply lookup_loc_extend_eq.
+      * eapply gt_allocptr_heap_lookup_none.
+        apply gt_allocptr_succ. exact Hgt_prev.
+    + assert (Hneq_lr : (l0, r0) <> (l, r)).
+      { intro Heq. apply HfreshN. rewrite Heq in HinN_old. exact HinN_old. }
+      destruct (Hwrite l0 r0 HinN_old) as [i0 [Hlk Hnone_cell]].
+      exists i0. split.
+      * rewrite lookup_loc_extend_neq.
+        -- exact Hlk.
+        -- exact Hneq_lr.
+      * exact Hnone_cell.
+  - intros r0 HinA.
+    simpl in HinA. destruct HinA as [Heq | HinA].
+    + inversion Heq.
+    + destruct (in_remove_alloc_region_inv _ _ _ _ HinA) as [HinA_old _].
+      eapply Hempty. exact HinA_old.
+  - intros r0 Hheap.
+    destruct (region_var_eq_dec r0 r) as [Heq | Hneq].
+    + subst. exists l. apply in_extend_alloc_new.
+    + destruct (Htracked r0 Hheap) as [l0 HinA].
+      exists l0. eapply in_extend_alloc_old; eauto.
+  - intros l0 r0 T HinSigma HinN.
+    destruct (in_extend_nursery_inv N (l, r) (l0, r0) HinN) as [Heq | HinN_old].
+    + apply HfreshS. rewrite <- Heq. eapply in_store_laddrs_of_entry. exact HinSigma.
+    + eapply Hdisj1; eauto.
+  - intros l0 r0 HinN HexSigma.
+    destruct (in_extend_nursery_inv N (l, r) (l0, r0) HinN) as [Heq | HinN_old].
+    + destruct HexSigma as [T HinSigma].
+      apply HfreshS. rewrite <- Heq. eapply in_store_laddrs_of_entry. exact HinSigma.
+    + eapply Hdisj2; eauto.
+Qed.
+
+Lemma store_wf_extend_letloc_after :
+  forall DI Sigma C A N M S l l1 r tc_prev i j,
+    store_wf DI Sigma C A N M S ->
+    letloc_fresh_ctx Sigma C A N (l, r) ->
+    In (r, AP_Loc (l1, r)) A ->
+    In ((l1, r), tc_prev) Sigma ->
+    ~ In (l1, r) N ->
+    lookup_loc M (l1, r) = Some (r, i) ->
+    end_witness DI S (r, i) tc_prev (r, j) ->
+    store_wf DI Sigma
+             (extend_conloc C (l, r) (LE_After tc_prev l1 r))
+             (extend_alloc A r (AP_Loc (l, r)))
+             (extend_nursery N (l, r))
+             (extend_loc M (l, r) (r, j))
+             S.
+Proof.
+  intros DI Sigma C A N M S l l1 r tc_prev i j
+         Hwf Hfresh Hfocus_prev Hstore_prev Hnotin_prev Hlookup_prev Hew_prev.
+  destruct Hfresh as [HfreshS [HfreshC [HfreshA HfreshN]]].
+  destruct Hwf as [Hmap [Hcfc [Halloc [Hdisj1 Hdisj2]]]].
+  destruct Hcfc as [Hstart [Hnext Hafter]].
+  destruct Halloc as [Hlin1 [Hlin2 [Hwrite [Hempty Htracked]]]].
+  assert (Hgt_prev : gt_allocptr j (allocptr S r)).
+  { eapply Hlin2; eauto. }
+  repeat split.
+  - intros l0 r0 T HinSigma.
+    destruct (Hmap l0 r0 T HinSigma) as [i0 [j0 [Hlk Hew]]].
+    exists i0, j0. split.
+    + rewrite lookup_loc_extend_neq.
+      * exact Hlk.
+      * intro Heq. apply HfreshS. rewrite <- Heq.
+        eapply in_store_laddrs_of_entry. exact HinSigma.
+    + exact Hew.
+  - intros l0 r0 HinC.
+    simpl in HinC. destruct HinC as [Heq | HinC].
+    + inversion Heq.
+    + rewrite lookup_loc_extend_neq.
+      * eapply Hstart. exact HinC.
+      * intro Heq. apply HfreshC. rewrite <- Heq.
+        eapply in_conloc_support_of_key. exact HinC.
+  - intros l0 r0 lprev HinC.
+    simpl in HinC. destruct HinC as [Heq | HinC].
+    + inversion Heq.
+    + destruct (Hnext l0 r0 lprev HinC) as [i0 [Hsrc Hdst]].
+      exists i0. split.
+      * rewrite lookup_loc_extend_neq.
+        -- exact Hsrc.
+        -- intro Heq. apply HfreshC. rewrite <- Heq.
+           eapply in_conloc_support_of_rhs
+             with (lr' := (l0, r0)) (le := LE_Next lprev r0).
+           ++ exact HinC.
+           ++ simpl. left. reflexivity.
+      * rewrite lookup_loc_extend_neq.
+        -- exact Hdst.
+        -- intro Heq. apply HfreshC. rewrite <- Heq.
+           eapply in_conloc_support_of_key. exact HinC.
+  - intros l0 r0 T l0' HinC.
+    simpl in HinC. destruct HinC as [Heq | HinC].
+    + inversion Heq; subst. exists i, j. repeat split.
+      * rewrite lookup_loc_extend_neq.
+        -- exact Hlookup_prev.
+        -- intro Heq_lr. apply HfreshA. rewrite <- Heq_lr.
+           eapply in_alloc_laddrs_of_entry. exact Hfocus_prev.
+      * exact Hew_prev.
+      * apply lookup_loc_extend_eq.
+    + destruct (Hafter l0 r0 T l0' HinC) as [i0 [j0 [Hsrc [Hew Hdst]]]].
+      exists i0, j0. repeat split.
+      * rewrite lookup_loc_extend_neq.
+        -- exact Hsrc.
+        -- intro Heq. apply HfreshC. rewrite <- Heq.
+           eapply in_conloc_support_of_rhs
+             with (lr' := (l0, r0)) (le := LE_After T l0' r0).
+           ++ exact HinC.
+           ++ simpl. left. reflexivity.
+      * exact Hew.
+      * rewrite lookup_loc_extend_neq.
+        -- exact Hdst.
+        -- intro Heq. apply HfreshC. rewrite <- Heq.
+           eapply in_conloc_support_of_key. exact HinC.
+  - intros r0 l0 HinA HinN.
+    simpl in HinA. destruct HinA as [Heq | HinA].
+    + inversion Heq; subst. exists j. split.
+      * apply lookup_loc_extend_eq.
+      * exact Hgt_prev.
+    + destruct (in_remove_alloc_region_inv _ _ _ _ HinA) as [HinA_old Hrneq].
+      assert (Hneq_lr : (l0, r0) <> (l, r)).
+      { intro Heq. inversion Heq; subst. contradiction. }
+      destruct (in_extend_nursery_inv N (l, r) (l0, r0) HinN) as [HeqN | HinN_old].
+      * inversion HeqN; subst. contradiction.
+      * destruct (Hlin1 r0 l0 HinA_old HinN_old) as [i0 [Hlk Hgt]].
+        exists i0. split.
+        -- rewrite lookup_loc_extend_neq.
+           ++ exact Hlk.
+           ++ exact Hneq_lr.
+        -- exact Hgt.
+  - intros r0 l0 i0 T j0 HinA Hlk Hnin Hew.
+    simpl in HinA. destruct HinA as [Heq | HinA].
+    + inversion Heq; subst. exfalso. apply Hnin. simpl. left. reflexivity.
+    + destruct (in_remove_alloc_region_inv _ _ _ _ HinA) as [HinA_old _].
+      assert (Hneq_lr : (l0, r0) <> (l, r)).
+      { intro Heq. apply HfreshA. rewrite <- Heq.
+        eapply in_alloc_laddrs_of_entry. exact HinA_old. }
+      destruct (not_in_extend_nursery_inv N (l, r) (l0, r0) Hnin) as [_ Hnin_old].
+      rewrite lookup_loc_extend_neq in Hlk by exact Hneq_lr.
+      eapply Hlin2; eauto.
+  - intros l0 r0 HinN.
+    destruct (in_extend_nursery_inv N (l, r) (l0, r0) HinN) as [Heq | HinN_old].
+    + inversion Heq; subst. exists j. split.
+      * apply lookup_loc_extend_eq.
+      * eapply gt_allocptr_heap_lookup_none. exact Hgt_prev.
+    + assert (Hneq_lr : (l0, r0) <> (l, r)).
+      { intro Heq. apply HfreshN. rewrite Heq in HinN_old. exact HinN_old. }
+      destruct (Hwrite l0 r0 HinN_old) as [i0 [Hlk Hnone_cell]].
+      exists i0. split.
+      * rewrite lookup_loc_extend_neq.
+        -- exact Hlk.
+        -- exact Hneq_lr.
+      * exact Hnone_cell.
+  - intros r0 HinA.
+    simpl in HinA. destruct HinA as [Heq | HinA].
+    + inversion Heq.
+    + destruct (in_remove_alloc_region_inv _ _ _ _ HinA) as [HinA_old _].
+      eapply Hempty. exact HinA_old.
+  - intros r0 Hheap.
+    destruct (region_var_eq_dec r0 r) as [Heq | Hneq].
+    + subst. exists l. apply in_extend_alloc_new.
+    + destruct (Htracked r0 Hheap) as [l0 HinA].
+      exists l0. eapply in_extend_alloc_old; eauto.
+  - intros l0 r0 T HinSigma HinN.
+    destruct (in_extend_nursery_inv N (l, r) (l0, r0) HinN) as [Heq | HinN_old].
+    + apply HfreshS. rewrite <- Heq. eapply in_store_laddrs_of_entry. exact HinSigma.
+    + eapply Hdisj1; eauto.
+  - intros l0 r0 HinN HexSigma.
+    destruct (in_extend_nursery_inv N (l, r) (l0, r0) HinN) as [Heq | HinN_old].
+    + destruct HexSigma as [T HinSigma].
+      apply HfreshS. rewrite <- Heq. eapply in_store_laddrs_of_entry. exact HinSigma.
+    + eapply Hdisj2; eauto.
+Qed.
+
+Lemma has_type_sigma_c_monotone :
+  (forall FDs DI G Sigma C A N A' N' e T,
+      has_type FDs DI G Sigma C A N A' N' e T ->
+      forall Sigma' C',
+        store_extends Sigma Sigma' ->
+        conloc_extends C C' ->
+        has_type FDs DI G Sigma' C' A N A' N' e T)
+  /\
+  (forall FDs DI tc_s G Sigma C A N A' N' T p,
+      pat_has_type FDs DI tc_s G Sigma C A N A' N' T p ->
+      forall Sigma' C',
+        store_extends Sigma Sigma' ->
+        conloc_extends C C' ->
+        pat_has_type FDs DI tc_s G Sigma' C' A N A' N' T p)
+  /\
+  (forall FDs DI tc_s G Sigma C A N A' N' T ps,
+      pats_have_type FDs DI tc_s G Sigma C A N A' N' T ps ->
+      forall Sigma' C',
+        store_extends Sigma Sigma' ->
+        conloc_extends C C' ->
+        pats_have_type FDs DI tc_s G Sigma' C' A N A' N' T ps).
+Proof.
+  eapply typing_mutind
+    with
+      (P0 := fun FDs DI G Sigma C A N r vs fields HT =>
+               forall Sigma' C',
+                 store_extends Sigma Sigma' ->
+                 conloc_extends C C' ->
+                 field_vals_have_type FDs DI G Sigma' C' A N r vs fields)
+      (P1 := fun FDs DI G Sigma C A N formals actuals vs params HT =>
+               forall Sigma' C',
+                 store_extends Sigma Sigma' ->
+                 conloc_extends C C' ->
+                 app_vals_have_type FDs DI G Sigma' C' A N formals actuals vs params).
+  - intros FDs DI G S0 C A N x tc l r Hlookup Hstore Sigma' C' Hse Hce.
+    apply T_Var.
+    + exact Hlookup.
+    + apply Hse. exact Hstore.
+  - intros FDs DI G S0 C A N r0 i l r tc Hstore Sigma' C' Hse Hce.
+    apply T_ConcreteLoc. apply Hse. exact Hstore.
+  - intros FDs DI G S0 C A N A' N' A'' N'' x e1 e2 tc1 l1 r1 tc2 l2 r2
+      Hty1 IH1 Hty2 IH2 Sigma' C' Hse Hce.
+    eapply T_Let.
+    + apply IH1; assumption.
+    + apply IH2.
+      * apply store_extends_extend_store. exact Hse.
+      * exact Hce.
+  - intros FDs DI G S0 C A N A' N' r e t Hfresh Hty IH Sigma' C' Hse Hce.
+    eapply T_LRegion.
+    + exact Hfresh.
+    + apply IH; assumption.
+  - intros FDs DI G S0 C A N A'' N'' l r e tc' l' r'
+      Halloc HfreshOut Hneq
+      Hty IH Sigma' C' Hse Hce.
+    eapply T_LLStart; eauto.
+    apply IH.
+    + exact Hse.
+    + apply conloc_extends_extend_conloc. exact Hce.
+  - intros FDs DI G S0 C A N A'' N'' l lprev r e tc'' l'' r''
+      Halloc Hnur HfreshOut Hneq Hty IH Sigma' C' Hse Hce.
+    eapply T_LLTag; eauto.
+    apply IH.
+    + exact Hse.
+    + apply conloc_extends_extend_conloc. exact Hce.
+  - intros FDs DI G S0 C A N A'' N'' l l1 r tc_prev e tc' l' r'
+      Halloc Hstore Hnotin HfreshOut Hneq
+      Hty IH Sigma' C' Hse Hce.
+    eapply T_LLAfter.
+    + exact Halloc.
+    + apply Hse. exact Hstore.
+    + exact Hnotin.
+    + exact HfreshOut.
+    + exact Hneq.
+    + apply IH.
+      * exact Hse.
+      * apply conloc_extends_extend_conloc. exact Hce.
+  - intros FDs DI G S0 C A N dc l r vs tc fieldtcs fields
+      Hdc Hnur Hfields Hlayout Hfocus Hvals IHvals Sigma' C' Hse Hce.
+    eapply T_DataCon.
+    + exact Hdc.
+    + exact Hnur.
+    + exact Hfields.
+    + apply constructor_layout_extends with (C := C); assumption.
+    + exact Hfocus.
+    + apply IHvals; assumption.
+  - intros FDs DI G S0 C A N f lrs vs tc l r f_locs f_params f_retty
+      f_regions f_body Hfd Hnur Halloc Hlen Hret Hargs IHargs Sigma' C' Hse Hce.
+    eapply T_App.
+    + exact Hfd.
+    + exact Hnur.
+    + exact Halloc.
+    + exact Hlen.
+    + exact Hret.
+    + apply IHargs; assumption.
+  - intros FDs DI G S0 C A N A' N' scrut ps tc_s l_s r_s t
+      Hscrut IHscrut Hcover Hps IHps Sigma' C' Hse Hce.
+    eapply T_Case.
+    + apply IHscrut; assumption.
+    + exact Hcover.
+    + apply IHps; assumption.
+  - intros FDs DI G S0 C A N r Sigma' C' Hse Hce.
+    apply T_FieldValsNil.
+  - intros FDs DI G S0 C A N r vl fld vs flds Hhead IHhead Htail IHtail
+      Sigma' C' Hse Hce.
+    eapply T_FieldValsCons.
+    + apply IHhead; assumption.
+    + apply IHtail; assumption.
+  - intros FDs DI G S0 C A N formals actuals Sigma' C' Hse Hce.
+    apply T_AppValsNil.
+  - intros FDs DI G S0 C A N formals actuals vl param vs params
+      Hhead IHhead Htail IHtail Sigma' C' Hse Hce.
+    eapply T_AppValsCons.
+    + apply IHhead; assumption.
+    + apply IHtail; assumption.
+  - intros FDs DI tc_s G S0 C A N A' N' dc binds body tc fieldtcs tc_res l r
+      Hdc Htc Hfields Hstore Hbody IHbody Sigma' C' Hse Hce.
+    eapply T_Pat.
+    + exact Hdc.
+    + exact Htc.
+    + exact Hfields.
+    + apply Hse. exact Hstore.
+    + eapply (IHbody (extend_store_list Sigma' (pat_store_entries binds)) C').
+      * apply store_extends_extend_store_list. exact Hse.
+      * exact Hce.
+  - intros FDs DI tc_s G S0 C A N t Sigma' C' Hse Hce.
+    apply T_PatsNil.
+  - intros FDs DI tc_s G S0 C A N A1 N1 A2 N2 t p ps Hpat IHpat Hps IHps
+      Sigma' C' Hse Hce.
+    eapply T_PatsCons.
+    + apply IHpat; assumption.
+    + apply IHps; assumption.
+Qed.
+
+Corollary expr_has_type_sigma_c_monotone :
+  forall FDs DI G Sigma C A N A' N' e T,
+    has_type FDs DI G Sigma C A N A' N' e T ->
+    forall Sigma' C',
+      store_extends Sigma Sigma' ->
+      conloc_extends C C' ->
+      has_type FDs DI G Sigma' C' A N A' N' e T.
+Proof.
+  intros. destruct has_type_sigma_c_monotone as [Hex _]. eauto.
+Qed.
+
+Corollary pat_has_type_sigma_c_monotone :
+  forall FDs DI tc_s G Sigma C A N A' N' T p,
+    pat_has_type FDs DI tc_s G Sigma C A N A' N' T p ->
+    forall Sigma' C',
+      store_extends Sigma Sigma' ->
+      conloc_extends C C' ->
+      pat_has_type FDs DI tc_s G Sigma' C' A N A' N' T p.
+Proof.
+  intros. destruct has_type_sigma_c_monotone as [_ [Hpat _]]. eauto.
+Qed.
+
+Corollary pats_have_type_sigma_c_monotone :
+  forall FDs DI tc_s G Sigma C A N A' N' T ps,
+    pats_have_type FDs DI tc_s G Sigma C A N A' N' T ps ->
+    forall Sigma' C',
+      store_extends Sigma Sigma' ->
+      conloc_extends C C' ->
+      pats_have_type FDs DI tc_s G Sigma' C' A N A' N' T ps.
+Proof.
+  intros. destruct has_type_sigma_c_monotone as [_ [_ Hps]]. eauto.
 Qed.
 
 Lemma existsb_bind_hit :
@@ -715,13 +1825,59 @@ Qed.
 (* Lemma: Substitution  (thesis Appendix A, Lemma Substitution)       *)
 (*                                                                    *)
 (* Substituting well-typed values for variables in a well-typed       *)
-(* expression preserves typing. This is currently the closed-value    *)
-(* version for the named-syntax mechanization. The full thesis lemma  *)
-(* is more general: it allows open values and simultaneous location   *)
-(* substitution under the thesis's unique-binder convention           *)
-(* (formalized in LoCalSyntax via expr_binders_unique,               *)
-(* fdecl_binders_unique, and program_binders_unique).                *)
+(* expression preserves typing. For the named-syntax mechanization,   *)
+(* open values require an explicit no-capture side condition.         *)
+(* The full thesis lemma is more general still: it is simultaneous    *)
+(* over value, location, and region substitution under the thesis's   *)
+(* global uniquify convention.                                        *)
 (* ================================================================= *)
+
+Fixpoint pats_bound_term_vars (ps : list pat) : list term_var :=
+  match ps with
+  | nil => nil
+  | p :: ps' => pat_bound_term_vars p ++ pats_bound_term_vars ps'
+  end.
+
+Lemma value_typing_extend_tenv_miss :
+  forall FDs DI G Sigma C A N vl T x tx,
+    has_type FDs DI G Sigma C A N A N (e_val vl) T ->
+    ~ In x (val_term_vars vl) ->
+    has_type FDs DI (extend_tenv G x tx) Sigma C A N A N (e_val vl) T.
+Proof.
+  intros FDs DI G Sigma C A N vl T x tx Hty Hmiss.
+  inversion Hty; subst; simpl in *.
+  - apply T_Var.
+    + simpl. destruct (term_var_eq_dec x0 x) as [Heq | Hneq].
+      * subst. exfalso. apply Hmiss. simpl. left. reflexivity.
+      * match goal with
+        | [ Hlk : lookup_tenv G x0 = Some _ |- _ ] => exact Hlk
+        end.
+    + match goal with
+      | [ Hstore : In ((l, r), tc) Sigma |- _ ] => exact Hstore
+      end.
+  - apply T_ConcreteLoc.
+    match goal with
+    | [ Hstore : In ((l, r), tc) Sigma |- _ ] => exact Hstore
+    end.
+Qed.
+
+Lemma value_typing_extend_tenv_list_disjoint :
+  forall FDs DI G Sigma C A N vl T binds,
+    has_type FDs DI G Sigma C A N A N (e_val vl) T ->
+    (forall x t, In (x, t) binds -> ~ In x (val_term_vars vl)) ->
+    has_type FDs DI (extend_tenv_list G binds) Sigma C A N A N (e_val vl) T.
+Proof.
+  intros FDs DI G Sigma C A N vl T binds Hty.
+  revert G Hty.
+  induction binds as [| [x t] binds IH]; intros G Hty Hdisj; simpl.
+  - exact Hty.
+  - apply IH.
+    + eapply value_typing_extend_tenv_miss.
+      * exact Hty.
+      * eapply Hdisj. left. reflexivity.
+    + intros y ty Hin.
+      eapply Hdisj. right. exact Hin.
+Qed.
 
 Definition subst_expr_case
     FDs DI G Sigma C A N A' N' e T
@@ -729,7 +1885,8 @@ Definition subst_expr_case
   forall prefix z uty Gamma s,
     G = ((prefix ++ (z, uty) :: Gamma)%list) ->
     lookup_tenv prefix z = None ->
-    has_type FDs DI nil Sigma C A N A N (e_val s) uty ->
+    has_type FDs DI (prefix ++ Gamma)%list Sigma C A N A N (e_val s) uty ->
+    (forall y, In y (val_term_vars s) -> ~ In y (expr_bound_term_vars e)) ->
     has_type FDs DI (prefix ++ Gamma)%list Sigma C A N A' N' (subst_val z s e) T.
 
 Definition subst_pat_case
@@ -738,7 +1895,8 @@ Definition subst_pat_case
   forall prefix z uty Gamma s,
     G = ((prefix ++ (z, uty) :: Gamma)%list) ->
     lookup_tenv prefix z = None ->
-    has_type FDs DI nil Sigma C A N A N (e_val s) uty ->
+    has_type FDs DI (prefix ++ Gamma)%list Sigma C A N A N (e_val s) uty ->
+    (forall y, In y (val_term_vars s) -> ~ In y (pat_bound_term_vars p)) ->
     pat_has_type FDs DI tc_s (prefix ++ Gamma)%list Sigma C A N A' N' T (subst_pat_val z s p).
 
 Definition subst_field_vals_case
@@ -747,7 +1905,7 @@ Definition subst_field_vals_case
   forall prefix z uty Gamma s,
     G = ((prefix ++ (z, uty) :: Gamma)%list) ->
     lookup_tenv prefix z = None ->
-    has_type FDs DI nil Sigma C A N A N (e_val s) uty ->
+    has_type FDs DI (prefix ++ Gamma)%list Sigma C A N A N (e_val s) uty ->
     field_vals_have_type FDs DI (prefix ++ Gamma)%list Sigma C A N r
       (List.map (subst_in_val z s) vs) fields.
 
@@ -757,7 +1915,7 @@ Definition subst_app_vals_case
   forall prefix z uty Gamma s,
     G = ((prefix ++ (z, uty) :: Gamma)%list) ->
     lookup_tenv prefix z = None ->
-    has_type FDs DI nil Sigma C A N A N (e_val s) uty ->
+    has_type FDs DI (prefix ++ Gamma)%list Sigma C A N A N (e_val s) uty ->
     app_vals_have_type FDs DI (prefix ++ Gamma)%list Sigma C A N formals actuals
       (List.map (subst_in_val z s) vs) params.
 
@@ -767,7 +1925,8 @@ Definition subst_pats_case
   forall prefix z uty Gamma s,
     G = ((prefix ++ (z, uty) :: Gamma)%list) ->
     lookup_tenv prefix z = None ->
-    has_type FDs DI nil Sigma C A N A N (e_val s) uty ->
+    has_type FDs DI (prefix ++ Gamma)%list Sigma C A N A N (e_val s) uty ->
+    (forall y, In y (val_term_vars s) -> ~ In y (pats_bound_term_vars ps)) ->
     pats_have_type FDs DI tc_s (prefix ++ Gamma)%list Sigma C A N A' N' T (subst_pats_val z s ps).
 
 Lemma substitution_val_mutual :
@@ -791,7 +1950,7 @@ Proof.
                subst_app_vals_case FDs DI G Sigma C A N formals actuals vs params HT).
   - intros FDs DI G Sigma C A N x tc l r Hlookup Hstore.
     unfold subst_expr_case.
-    intros prefix z uty Gamma s HG Hnone Hclosed.
+    intros prefix z uty Gamma s HG Hnone Hs Hfresh.
     subst G. simpl in *.
     rewrite lookup_tenv_app in Hlookup.
     destruct (lookup_tenv prefix x) eqn:Hprefix.
@@ -805,9 +1964,7 @@ Proof.
       destruct (term_var_eq_dec x z) as [Heq | Hneq].
       * subst x. inversion Hlookup; subst.
         simpl. destruct (term_var_eq_dec z z); [| contradiction].
-        eapply closed_value_typing_any_context.
-        -- exact Hclosed.
-        -- intros lr tc' Hin. exact Hin.
+        exact Hs.
       * simpl. destruct (term_var_eq_dec z x) as [Heqzx | Hneqzx].
         { exfalso. apply Hneq. symmetry. exact Heqzx. }
         apply T_Var.
@@ -816,13 +1973,17 @@ Proof.
         -- exact Hstore.
   - intros FDs DI G Sigma C A N r0 i l r tc Hstore.
     unfold subst_expr_case.
-    intros prefix z uty Gamma s HG Hnone Hclosed.
+    intros prefix z uty Gamma s HG Hnone Hs Hfresh.
     subst G. simpl. apply T_ConcreteLoc. exact Hstore.
   - intros FDs DI G Sigma C A N A' N' A'' N'' x e1 e2 tc1 l1 r1 tc2 l2 r2
       Hty1 IH1 Hty2 IH2.
     unfold subst_expr_case.
-    intros prefix z uty Gamma s HG Hnone Hclosed.
+    intros prefix z uty Gamma s HG Hnone Hs Hfresh.
     subst G. simpl.
+    assert (Hfresh_e1 :
+      forall y, In y (val_term_vars s) -> ~ In y (expr_bound_term_vars e1)).
+    { intros y Hy Hin.
+      apply (Hfresh y Hy). simpl. apply in_or_app. left. exact Hin. }
     eapply T_Let.
     + eapply IH1; eauto.
     + destruct (term_var_eq_dec z x) as [Heq | Hneq].
@@ -835,93 +1996,124 @@ Proof.
            apply tenv_equiv_shadow_under_prefix.
            simpl. destruct (term_var_eq_dec z z); [discriminate | contradiction].
       * simpl.
+        assert (Hs_mid :
+          has_type FDs DI (((x, LocTy tc1 l1 r1) :: prefix ++ Gamma)%list)
+                   Sigma C A N A N (e_val s) uty).
+        { change (((x, LocTy tc1 l1 r1) :: prefix ++ Gamma)%list)
+            with (extend_tenv ((prefix ++ Gamma)%list) x (LocTy tc1 l1 r1)).
+          eapply value_typing_extend_tenv_miss.
+          - exact Hs.
+          - intro Hinx.
+            apply (Hfresh x Hinx).
+            simpl. apply in_or_app. right. simpl. left. reflexivity.
+        }
+        assert (Hs_ext :
+          has_type FDs DI (((x, LocTy tc1 l1 r1) :: prefix ++ Gamma)%list)
+                   (extend_store Sigma (l1, r1) tc1) C A' N' A' N' (e_val s) uty).
+        { eapply value_typing_any_context.
+          - exact Hs_mid.
+          - intros y. reflexivity.
+          - intros lr tc' Hin. simpl. right. exact Hin.
+        }
         eapply IH2
           with (prefix := (x, LocTy tc1 l1 r1) :: prefix)
                (z := z) (uty := uty) (Gamma := Gamma) (s := s).
         -- reflexivity.
         -- simpl. destruct (term_var_eq_dec z x); [contradiction | exact Hnone].
-        -- eapply closed_value_typing_any_context.
-           ++ exact Hclosed.
-           ++ intros lr tc' Hin. simpl. right. exact Hin.
-  - intros FDs DI G Sigma C A N A' N' r e t Hty IH.
+        -- exact Hs_ext.
+        -- intros y Hy Hin.
+           apply (Hfresh y Hy).
+           simpl. apply in_or_app. right. simpl. right. exact Hin.
+  - intros FDs DI G Sigma C A N A' N' r e t Hfresh Hty IH.
     unfold subst_expr_case.
-    intros prefix z uty Gamma s HG Hnone Hclosed.
+    intros prefix z uty Gamma s HG Hnone Hs Hfresh_s.
     subst G. simpl.
     eapply T_LRegion.
-    eapply IH; eauto.
-    eapply closed_value_typing_any_context.
-    + exact Hclosed.
-    + intros lr tc' Hin. exact Hin.
-  - intros FDs DI G Sigma C A N A'' N'' l r e tc' l' r' Halloc Hfresh Hneq
-      Hty IH.
+    + exact Hfresh.
+    + eapply IH; eauto.
+      eapply value_typing_any_context.
+      * exact Hs.
+      * intros y. reflexivity.
+      * intros lr tc' Hin. exact Hin.
+  - intros FDs DI G Sigma C A N A'' N'' l r e tc' l' r'
+      Halloc HfreshOut Hneq Hty IH.
     unfold subst_expr_case.
-    intros prefix z uty Gamma s HG Hnone Hclosed.
+    intros prefix z uty Gamma s HG Hnone Hs Hfresh_s.
     subst G. simpl.
     eapply T_LLStart; eauto.
     eapply IH; eauto.
-    eapply closed_value_typing_any_context.
-    + exact Hclosed.
+    eapply value_typing_any_context.
+    + exact Hs.
+    + intros y. reflexivity.
     + intros lr tc'' Hin. exact Hin.
   - intros FDs DI G Sigma C A N A'' N'' l lprev r e tc'' l'' r''
-      Halloc Hnur Hfresh Hneq Hty IH.
+      Halloc Hnur HfreshOut Hneq Hty IH.
     unfold subst_expr_case.
-    intros prefix z uty Gamma s HG Hnone Hclosed.
+    intros prefix z uty Gamma s HG Hnone Hs Hfresh_s.
     subst G. simpl.
     eapply T_LLTag; eauto.
     eapply IH; eauto.
-    eapply closed_value_typing_any_context.
-    + exact Hclosed.
+    eapply value_typing_any_context.
+    + exact Hs.
+    + intros y. reflexivity.
     + intros lr tc' Hin. exact Hin.
   - intros FDs DI G Sigma C A N A'' N'' l l1 r tc_prev e tc' l' r'
-      Halloc Hstore Hnotin Hfresh Hneq Hty IH.
+      Halloc Hstore Hnotin HfreshOut Hneq Hty IH.
     unfold subst_expr_case.
-    intros prefix z uty Gamma s HG Hnone Hclosed.
+    intros prefix z uty Gamma s HG Hnone Hs Hfresh_s.
     subst G. simpl.
     eapply T_LLAfter; eauto.
     eapply IH; eauto.
-    eapply closed_value_typing_any_context.
-    + exact Hclosed.
+    eapply value_typing_any_context.
+    + exact Hs.
+    + intros y. reflexivity.
     + intros lr tc'' Hin. exact Hin.
   - intros FDs DI G Sigma C A N dc l r vs tc fieldtcs fields
       Hdc Hnur Hfields Hlayout Hfocus Hvals IHvals.
     unfold subst_expr_case.
-    intros prefix z uty Gamma s HG Hnone Hclosed.
+    intros prefix z uty Gamma s HG Hnone Hs Hfresh.
     subst G. simpl.
     eapply T_DataCon; eauto.
   - intros FDs DI G Sigma C A N f lrs vs tc l r f_locs f_params f_retty
       f_regions f_body Hfd Hnur Halloc Hlen1 Hlen2 Hargs IHargs.
     unfold subst_expr_case.
-    intros prefix z uty Gamma s HG Hnone Hclosed.
+    intros prefix z uty Gamma s HG Hnone Hs Hfresh.
     subst G. simpl.
     eapply T_App; eauto.
   - intros FDs DI G Sigma C A N A' N' scrut ps tc_s l_s r_s t
       Hscrut IHscrut Hcover Hps IHps.
     unfold subst_expr_case.
-    intros prefix z uty Gamma s HG Hnone Hclosed.
+    intros prefix z uty Gamma s HG Hnone Hs Hfresh.
     subst G. rewrite subst_val_case.
+    assert (Hfresh_scrut :
+      forall y, In y (val_term_vars s) -> ~ In y (expr_bound_term_vars (e_val scrut))).
+    { intros y Hy Hin. simpl in Hin. contradiction. }
+    assert (Hfresh_ps :
+      forall y, In y (val_term_vars s) -> ~ In y (pats_bound_term_vars ps)).
+    { intros y Hy Hin. apply (Hfresh y Hy). simpl. exact Hin. }
     eapply T_Case.
     + eapply IHscrut; eauto.
     + eapply pats_cover_subst_pats_val. exact Hcover.
     + eapply IHps; eauto.
   - intros FDs DI G Sigma C A N r.
     unfold subst_field_vals_case.
-    intros prefix z uty Gamma s HG Hnone Hclosed.
+    intros prefix z uty Gamma s HG Hnone Hs.
     subst G. simpl. constructor.
   - intros FDs DI G Sigma C A N r vl fld vs flds Hhead IHhead Htail IHtail.
     unfold subst_field_vals_case.
-    intros prefix z uty Gamma s HG Hnone Hclosed.
+    intros prefix z uty Gamma s HG Hnone Hs.
     subst G. simpl.
     eapply T_FieldValsCons.
     + eapply IHhead; eauto.
     + eapply IHtail; eauto.
   - intros FDs DI G Sigma C A N formals actuals.
     unfold subst_app_vals_case.
-    intros prefix z uty Gamma s HG Hnone Hclosed.
+    intros prefix z uty Gamma s HG Hnone Hs.
     subst G. simpl. constructor.
   - intros FDs DI G Sigma C A N formals actuals vl param vs params
       Hhead IHhead Htail IHtail.
     unfold subst_app_vals_case.
-    intros prefix z uty Gamma s HG Hnone Hclosed.
+    intros prefix z uty Gamma s HG Hnone Hs.
     subst G. simpl.
     eapply T_AppValsCons.
     + eapply IHhead; eauto.
@@ -929,7 +2121,7 @@ Proof.
   - intros FDs DI tc_s G Sigma C A N A' N' dc binds body tc fieldtcs tc_res l r
       Hdc Htc Hfields Hstore Hbody IHbody.
     unfold subst_pat_case.
-    intros prefix z uty Gamma s HG Hnone Hclosed.
+    intros prefix z uty Gamma s HG Hnone Hs Hfresh.
     subst G. simpl.
     destruct
       (existsb
@@ -963,36 +2155,285 @@ Proof.
         -- repeat rewrite extend_tenv_list_rev.
            rewrite <- app_assoc. reflexivity.
         -- apply lookup_tenv_extend_tenv_list_miss; assumption.
-        -- eapply closed_value_typing_any_context.
-           ++ exact Hclosed.
+        -- eapply value_typing_any_context.
+           ++ eapply value_typing_extend_tenv_list_disjoint.
+              ** exact Hs.
+              ** intros x t HinBind Hinx.
+                 apply (Hfresh x Hinx). simpl. apply in_or_app. left.
+                 change (In x (pat_term_vars binds)).
+                 eapply in_map with (f := fst) in HinBind.
+                 exact HinBind.
+           ++ intros y.
+              repeat rewrite extend_tenv_list_rev.
+              rewrite <- app_assoc.
+              reflexivity.
            ++ intros ent tc' Hin. apply in_extend_store_list. exact Hin.
+        -- intros y Hy HinBody.
+           apply (Hfresh y Hy). simpl. apply in_or_app. right. exact HinBody.
       * repeat rewrite extend_tenv_list_rev.
         rewrite <- app_assoc. reflexivity.
   - intros FDs DI tc_s G Sigma C A N t.
     unfold subst_pats_case.
-    intros prefix z uty Gamma s HG Hnone Hclosed.
+    intros prefix z uty Gamma s HG Hnone Hs Hfresh.
     subst G. simpl. constructor.
   - intros FDs DI tc_s G Sigma C A N A1 N1 A2 N2 t p ps Hpat IHpat Hps IHps.
     unfold subst_pats_case.
-    intros prefix z uty Gamma s HG Hnone Hclosed.
+    intros prefix z uty Gamma s HG Hnone Hs Hfresh.
     subst G. simpl.
     eapply T_PatsCons.
     + eapply IHpat; eauto.
-    + eapply IHps; eauto.
-      eapply closed_value_typing_any_context.
-      * exact Hclosed.
-      * intros lr tc' Hin. exact Hin.
+      intros y Hy HinPat.
+      apply (Hfresh y Hy). simpl. apply in_or_app. left. exact HinPat.
+    + eapply IHps.
+      * reflexivity.
+      * exact Hnone.
+      * eapply value_typing_any_context.
+        -- exact Hs.
+        -- intros y. reflexivity.
+        -- intros lr tc' Hin. exact Hin.
+      * intros y Hy HinPs.
+        apply (Hfresh y Hy). simpl. apply in_or_app. right. exact HinPs.
 Qed.
 
 Lemma substitution_val :
   forall FDs DI Gamma x vty Sigma C A N A' N' e T v0,
     has_type FDs DI (cons (x, vty) Gamma) Sigma C A N A' N' e T ->
-    has_type FDs DI nil Sigma C A N A N (e_val v0) vty ->
+    has_type FDs DI Gamma Sigma C A N A N (e_val v0) vty ->
+    (forall y, In y (val_term_vars v0) -> ~ In y (expr_bound_term_vars e)) ->
     has_type FDs DI Gamma Sigma C A N A' N' (subst_val x v0 e) T.
 Proof.
-  intros FDs DI Gamma x vty Sigma C A N A' N' e T v0 HT Hclosed.
+  intros FDs DI Gamma x vty Sigma C A N A' N' e T v0 HT Hs Hfresh.
   destruct substitution_val_mutual as [Hex _].
   eapply Hex with (prefix := nil) (z := x) (uty := vty) (Gamma := Gamma) (s := v0); eauto.
+Qed.
+
+Lemma preservation_let_val_case :
+  forall FDs DI Sigma C A N Aout Nout M S x T1 vl e2 T,
+    has_type FDs DI nil Sigma C A N Aout Nout (e_let x T1 (e_val vl) e2) T ->
+    store_wf DI Sigma C A N M S ->
+    exists Sigma' C' Ain' Nin',
+      has_type FDs DI nil Sigma' C' Ain' Nin' Aout Nout
+               (subst_val x vl e2) T
+      /\ store_wf DI Sigma' C' Ain' Nin' M S
+      /\ store_extends Sigma Sigma'
+      /\ conloc_extends C C'.
+Proof.
+  intros FDs DI Sigma C A N Aout Nout M S x T1 vl e2 T Hty Hwf.
+  inversion Hty; subst.
+  destruct (has_type_value_same_io _ _ _ _ _ _ _ _ _ _ _ H13) as [HA' HN'].
+  subst A' N'.
+  inversion H13; subst.
+  - simpl in H11. discriminate.
+  - exists (extend_store Sigma (l1, r1) tc1), C, A, N.
+    split.
+    + eapply substitution_val.
+      * exact H14.
+      * apply T_ConcreteLoc. simpl. auto.
+      * intros y Hy. inversion Hy.
+    + split.
+      * eapply store_wf_extend_store_existing.
+        -- exact Hwf.
+        -- exact H10.
+      * split.
+        -- intros lr tc Hin. right. exact Hin.
+        -- apply conloc_extends_refl.
+Qed.
+
+Lemma preservation_letregion_case :
+  forall FDs DI Sigma C A N Aout Nout M S r body T,
+    has_type FDs DI nil Sigma C A N Aout Nout (e_letregion r body) T ->
+    store_wf DI Sigma C A N M S ->
+    exists Sigma' C' Ain' Nin',
+      has_type FDs DI nil Sigma' C' Ain' Nin' Aout Nout body T
+      /\ store_wf DI Sigma' C' Ain' Nin' M S
+      /\ store_extends Sigma Sigma'
+      /\ conloc_extends C C'.
+Proof.
+  intros FDs DI Sigma C A N Aout Nout M S r body T Hty Hwf.
+  inversion Hty; subst.
+  exists Sigma, C, (extend_alloc A r AP_None), N.
+  split.
+  - exact H12.
+  - split.
+    + eapply store_wf_extend_alloc_none_fresh; eauto.
+    + split.
+      * apply store_extends_refl.
+      * apply conloc_extends_refl.
+Qed.
+
+Lemma preservation_letloc_start_case :
+  forall FDs DI Sigma C A N Aout Nout M S l r body T,
+    has_type FDs DI nil Sigma C A N Aout Nout
+             (e_letloc l r (LE_Start r) body) T ->
+    has_type_fresh FDs DI nil Sigma C A N Aout Nout
+                    (e_letloc l r (LE_Start r) body) T ->
+    store_wf DI Sigma C A N M S ->
+    exists Sigma' C' Ain' Nin',
+      has_type FDs DI nil Sigma' C' Ain' Nin' Aout Nout body T
+      /\ store_wf DI Sigma' C' Ain' Nin' (extend_loc M (l, r) (r, 0)) S
+      /\ store_extends Sigma Sigma'
+      /\ conloc_extends C C'.
+Proof.
+  intros FDs DI Sigma C A N Aout Nout M S l r body T Hty Hfresh Hwf.
+  inversion Hty; subst. clear Hty.
+  inversion Hfresh; subst. clear Hfresh.
+  exists Sigma,
+         (extend_conloc C (l, r) (LE_Start r)),
+         (extend_alloc A r (AP_Loc (l, r))),
+         (extend_nursery N (l, r)).
+  split.
+  - match goal with
+    | [ Hbody : has_type _ _ _ _ _ _ _ _ _ body _ |- _ ] => exact Hbody
+    end.
+  - split.
+    + eapply store_wf_extend_letloc_start; eauto.
+    + split.
+      * apply store_extends_refl.
+      * intros lr le Hin.
+        simpl. right. exact Hin.
+Qed.
+
+Lemma preservation_letloc_tag_case :
+  forall FDs DI Sigma C A N Aout Nout M S l lprev r body T rc i,
+    has_type FDs DI nil Sigma C A N Aout Nout
+             (e_letloc l r (LE_Next lprev r) body) T ->
+    has_type_fresh FDs DI nil Sigma C A N Aout Nout
+                    (e_letloc l r (LE_Next lprev r) body) T ->
+    store_wf DI Sigma C A N M S ->
+    lookup_loc M (lprev, r) = Some (rc, i) ->
+    exists Sigma' C' Ain' Nin',
+      has_type FDs DI nil Sigma' C' Ain' Nin' Aout Nout body T
+      /\ store_wf DI Sigma' C' Ain' Nin' (extend_loc M (l, r) (rc, i + 1)) S
+      /\ store_extends Sigma Sigma'
+      /\ conloc_extends C C'.
+Proof.
+  intros FDs DI Sigma C A N Aout Nout M S l lprev r body T rc i
+         Hty Hfresh Hwf Hlookup.
+  inversion Hty; subst; clear Hty.
+  inversion Hfresh; subst; clear Hfresh.
+  pose proof Hwf as Hwf_copy.
+  destruct Hwf_copy as [_ [_ [Halloc _]]].
+  destruct Halloc as [Hlin1 _].
+  match goal with
+  | [ Hfocus : In (r, AP_Loc (lprev, r)) A,
+      Hnur : In (lprev, r) N |- _ ] =>
+      destruct (Hlin1 r lprev Hfocus Hnur) as [i0 [Hlk0 Hgt0]]
+  end.
+  rewrite Hlookup in Hlk0. inversion Hlk0; subst rc i0.
+  exists Sigma,
+         (extend_conloc C (l, r) (LE_Next lprev r)),
+         (extend_alloc A r (AP_Loc (l, r))),
+         (extend_nursery N (l, r)).
+  split.
+  - match goal with
+    | [ Hbody : has_type _ _ _ _ _ _ _ _ _ body _ |- _ ] => exact Hbody
+    end.
+  - split.
+    + eapply store_wf_extend_letloc_tag; eauto.
+    + split.
+      * apply store_extends_refl.
+      * intros lr le Hin.
+        simpl. right. exact Hin.
+Qed.
+
+Lemma preservation_letloc_after_case :
+  forall FDs DI Sigma C A N Aout Nout M S l l1 r tc_prev body T rc i j,
+    has_type FDs DI nil Sigma C A N Aout Nout
+             (e_letloc l r (LE_After tc_prev l1 r) body) T ->
+    has_type_fresh FDs DI nil Sigma C A N Aout Nout
+                    (e_letloc l r (LE_After tc_prev l1 r) body) T ->
+    store_wf DI Sigma C A N M S ->
+    lookup_loc M (l1, r) = Some (rc, i) ->
+    end_witness DI S (rc, i) tc_prev (rc, j) ->
+    exists Sigma' C' Ain' Nin',
+      has_type FDs DI nil Sigma' C' Ain' Nin' Aout Nout body T
+      /\ store_wf DI Sigma' C' Ain' Nin' (extend_loc M (l, r) (rc, j)) S
+      /\ store_extends Sigma Sigma'
+      /\ conloc_extends C C'.
+Proof.
+  intros FDs DI Sigma C A N Aout Nout M S l l1 r tc_prev body T rc i j
+         Hty Hfresh Hwf Hlookup Hew.
+  inversion Hty; subst; clear Hty.
+  inversion Hfresh; subst; clear Hfresh.
+  pose proof Hwf as Hwf_copy.
+  destruct Hwf_copy as [Hmap _].
+  match goal with
+  | [ Hstore_prev : In ((l1, r), tc_prev) Sigma |- _ ] =>
+      destruct (Hmap l1 r tc_prev Hstore_prev) as [i0 [j0 [Hlk0 Hew0]]]
+  end.
+  rewrite Hlookup in Hlk0. inversion Hlk0; subst rc i0.
+  exists Sigma,
+         (extend_conloc C (l, r) (LE_After tc_prev l1 r)),
+         (extend_alloc A r (AP_Loc (l, r))),
+         (extend_nursery N (l, r)).
+  split.
+  - match goal with
+    | [ Hbody : has_type _ _ _ _ _ _ _ _ _ body _ |- _ ] => exact Hbody
+    end.
+  - split.
+    + eapply store_wf_extend_letloc_after; eauto.
+    + split.
+      * apply store_extends_refl.
+      * intros lr le Hin.
+        simpl. right. exact Hin.
+Qed.
+
+Lemma preserve_let_under_step :
+  forall FDs DI Sigma C A' N' Aout Nout
+         Sigma' C' Ain' Nin'
+         x tc1 l1 r1 e1' e2 tc2 l2 r2,
+    has_type FDs DI nil Sigma' C' Ain' Nin' A' N' e1'
+             (LocTy tc1 l1 r1) ->
+    has_type FDs DI (extend_tenv nil x (LocTy tc1 l1 r1))
+             (extend_store Sigma (l1, r1) tc1)
+             C A' N' Aout Nout e2 (LocTy tc2 l2 r2) ->
+    store_extends Sigma Sigma' ->
+    conloc_extends C C' ->
+    has_type FDs DI nil Sigma' C' Ain' Nin' Aout Nout
+             (e_let x (LocTy tc1 l1 r1) e1' e2) (LocTy tc2 l2 r2).
+Proof.
+  intros FDs DI Sigma C A' N' Aout Nout
+         Sigma' C' Ain' Nin'
+         x tc1 l1 r1 e1' e2 tc2 l2 r2 He1 Hbody Hse Hce.
+  eapply T_Let.
+  - exact He1.
+  - eapply expr_has_type_sigma_c_monotone.
+    + exact Hbody.
+    + apply store_extends_extend_store. exact Hse.
+    + exact Hce.
+Qed.
+
+Lemma preservation_let_expr_case :
+  forall FDs DI Sigma C A' N' Aout Nout
+         Sigma' C' Ain' Nin'
+         M' S'
+         x tc1 l1 r1 e1' e2 tc2 l2 r2,
+    has_type FDs DI nil Sigma' C' Ain' Nin' A' N' e1'
+             (LocTy tc1 l1 r1) ->
+    has_type FDs DI (extend_tenv nil x (LocTy tc1 l1 r1))
+             (extend_store Sigma (l1, r1) tc1)
+             C A' N' Aout Nout e2 (LocTy tc2 l2 r2) ->
+    store_wf DI Sigma' C' Ain' Nin' M' S' ->
+    store_extends Sigma Sigma' ->
+    conloc_extends C C' ->
+    exists Sigma'' C'' Ain'' Nin'',
+      has_type FDs DI nil Sigma'' C'' Ain'' Nin'' Aout Nout
+               (e_let x (LocTy tc1 l1 r1) e1' e2) (LocTy tc2 l2 r2)
+      /\ store_wf DI Sigma'' C'' Ain'' Nin'' M' S'
+      /\ store_extends Sigma Sigma''
+      /\ conloc_extends C C''.
+Proof.
+  intros FDs DI Sigma C A' N' Aout Nout
+         Sigma' C' Ain' Nin'
+         M' S'
+         x tc1 l1 r1 e1' e2 tc2 l2 r2
+         He1 Hbody Hwf Hse Hce.
+  exists Sigma', C', Ain', Nin'.
+  split.
+  - eapply preserve_let_under_step; eauto.
+  - split.
+    + exact Hwf.
+    + split; assumption.
 Qed.
 
 (* ================================================================= *)
@@ -1062,7 +2503,8 @@ Proof.
      M(lprev,r) = ⟨r,i⟩, so D_LetLoc_Tag applies. *)
   1: {
     right.
-    destruct Hwf as [_ [_ [[_ [_ [Hwo _]]] _]]].
+    destruct Hwf as [_ [_ [Halloc _]]].
+    destruct Halloc as [_ [_ [Hwo _]]].
     destruct (Hwo lprev r H0) as [i [Hlk _]].
     do 3 eexists. eapply D_LetLoc_Tag. exact Hlk.
   }
@@ -1082,7 +2524,8 @@ Proof.
      M(l,r) = ⟨r,i⟩, so D_DataCon applies. *)
   1: {
     right.
-    destruct Hwf as [_ [_ [[_ [_ [Hwo _]]] _]]].
+    destruct Hwf as [_ [_ [Halloc _]]].
+    destruct Halloc as [_ [_ [Hwo _]]].
     destruct (Hwo l r H0) as [i [Hlk _]].
     do 3 eexists. eapply D_DataCon. exact Hlk.
   }
@@ -1170,29 +2613,32 @@ Proof.
 Qed.
 
 (* ================================================================= *)
-(* Theorem: Preservation  (thesis §2.2.3, Lemma Preservation)        *)
+(* Theorem: Preservation  (mechanized restatement of thesis §2.2.3)  *)
 (*                                                                    *)
-(* If a well-typed expression takes a step under a well-formed store, *)
-(* the result is well-typed under (possibly extended) environments    *)
-(* and the new store remains well-formed.                             *)
+(* The thesis statement reuses A'/N' as though the reduct were always *)
+(* typed under the output environments of the source expression.      *)
+(* That is not true for this judgmental presentation: rules such as   *)
+(* T_Let, T_LLStart/T_LLTag/T_LLAfter, and T_Case step to subterms    *)
+(* whose typing lives under intermediate premise environments.        *)
 (*                                                                    *)
-(*   If  ∅;Σ;C;A;N ⊢ A';N'; e : T                                  *)
-(*   and store_wf(DI, Σ, C, A, N, M, S)                              *)
-(*   and S;M;e ⇒ S';M';e'                                           *)
-(*   then ∃ Σ'⊇Σ, C',                                               *)
-(*     ∅;Σ';C';A';N' ⊢ A'';N''; e' : T                              *)
-(*     and store_wf(DI, Σ', C', A', N', M', S')                      *)
+(* So the mechanized preservation lemma returns the reduct together   *)
+(* with the input environments it actually inhabits, while keeping    *)
+(* the source judgment's output environments fixed.  This is the      *)
+(* shape needed to rebuild enclosing rules like T_Let.                *)
 (* ================================================================= *)
 
 Theorem preservation :
-  forall FDs DI Sigma C A N A' N' M S e T S' M' e',
-    has_type FDs DI nil Sigma C A N A' N' e T ->
+  forall FDs DI Sigma C A N Aout Nout M S e T S' M' e',
+    Forall (fdecl_has_type FDs DI) FDs ->
+    has_type FDs DI nil Sigma C A N Aout Nout e T ->
+    has_type_fresh FDs DI nil Sigma C A N Aout Nout e T ->
     store_wf DI Sigma C A N M S ->
     step FDs DI S M e S' M' e' ->
-    exists Sigma' C' A'' N'',
-      has_type FDs DI nil Sigma' C' A' N' A'' N'' e' T
-      /\ store_wf DI Sigma' C' A' N' M' S'
-      /\ (forall lr T0, In (lr, T0) Sigma -> In (lr, T0) Sigma').
+    exists Sigma' C' Ain' Nin',
+      has_type FDs DI nil Sigma' C' Ain' Nin' Aout Nout e' T
+      /\ store_wf DI Sigma' C' Ain' Nin' M' S'
+      /\ store_extends Sigma Sigma'
+      /\ conloc_extends C C'.
 Proof.
   (* By rule induction on the step derivation.
      Key cases:
@@ -1218,7 +2664,7 @@ Proof.
          Store WF unchanged (S, M not modified).
 
        D_Let_Expr —
-         IH on sub-expression step.
+         IH on the stepped sub-expression, then rebuild T_Let.
 
        D_Case —
          Σ' extended with field location types.
@@ -1227,7 +2673,7 @@ Proof.
            get end-witness from scrutinee's end-witness.
 
        D_App —
-         Apply substitution lemma (values + locations).
+         Apply substitution/value-location instantiation for the callee body.
          Store WF unchanged.
 
        D_LetRegion —
@@ -1248,7 +2694,9 @@ Admitted.
 
 Theorem type_safety :
   forall FDs DI Sigma C A N A' N' M S e T Sn Mn en,
+    Forall (fdecl_has_type FDs DI) FDs ->
     has_type FDs DI nil Sigma C A N A' N' e T ->
+    has_type_fresh FDs DI nil Sigma C A N A' N' e T ->
     store_wf DI Sigma C A N M S ->
     di_functional DI ->
     expr_wf M e ->
